proofs/lang/low_memory.v
@@ -76,9 +76,7 @@ Proof. by rewrite /top_stack => s; rewrite (ss_frames s) (ss_root s). Qed.
 Lemma read_mem_valid_pointer m ptr sz w :
   read_mem m ptr sz = ok w ->
   valid_pointer m ptr sz.
-Proof.
-  by move => hr; apply /Memory.readV;exists w.
-Qed.
+Proof. apply /Memory.readV. Qed.
 
 Lemma write_mem_valid_pointer m ptr sz w m' :
   write_mem m ptr sz w = ok m' ->
@@ -86,11 +84,6 @@ Lemma write_mem_valid_pointer m ptr sz w m' :
 Proof.
   move => hw; apply /Memory.writeV; exists m'; exact hw.
 Qed.
-
-Lemma write_mem_can_read m ptr sz w m' :
-  write_mem m ptr sz w = ok m' ->
-  exists w', read_mem m ptr sz = ok w'.
-Proof. by move => /write_mem_valid_pointer /Memory.readV. Qed.
 
 Lemma alloc_stack_top_stack m ws sz sz' m' :
   alloc_stack m ws sz sz' = ok m' →
